Variant of own keyed by namespaces.

nsl.v
@@ -2,7 +2,9 @@ From stdpp Require Import base gmap.
 From mathcomp Require Import ssreflect.
 From iris.algebra Require Import agree auth csum gset gmap excl frac.
 From iris.heap_lang Require Import notation proofmode.
-From cryptis Require Import lib term cryptis primitives tactics session.
+From cryptis Require Import lib term cryptis primitives tactics role nown.
+From cryptis Require Import pk_auth.
+From cryptis Require Import session.
 
 Set Implicit Arguments.
 Unset Strict Implicit.
@@ -10,350 +12,80 @@ Unset Printing Implicit Defensive.
 
 Section NSL.
 
-Context `{!heapGS Σ, !cryptisG Σ}.
-Context `{TermMeta Σ term_meta term_meta_token}.
-Context `{!sessionG Σ}.
+Context `{heap : !heapGS Σ, cryptis : !cryptisG Σ, sess : !session.sessionG Σ}.
 Notation iProp := (iProp Σ).
-Implicit Types t : term.
-
-Definition corruption kA kB : iProp :=
-  pterm (TKey Dec kA) ∨ pterm (TKey Dec kB).
-
-Global Instance corruptionC : Comm (⊣⊢) corruption.
-Proof. by move=> k k'; rewrite /corruption [(_ ∨ _)%I]comm. Qed.
+Implicit Types t kI kR nI nR : term.
 
 Variable N : namespace.
 
-Variable P Q : role → term → term → term → term → iProp.
+Definition nsl_gen_keys : val := λ: <>,
+  let: "n" := mknonce #() in
+  ("n", "n").
 
-Definition nsl_sess_inv rl (tI tR : term) (m : term * term) : iProp :=
-  let '(kA, kB) := m in P rl tI tR kA kB.
+Definition nsl_mk_sess_key : val := λ: "nI" <>, "nI".
 
-Definition msg1_pred (kB : term) m1 : iProp :=
-  ∃ nA kA, ⌜m1 = Spec.of_list [nA; TKey Enc kA]⌝ ∧
-           (pterm nA ↔ ▷ corruption kA kB) ∧
-           pterm (TKey Enc kA).
+Definition nsl_init : expr :=
+  pk_auth_init N nsl_gen_keys nsl_mk_sess_key.
 
-Definition msg2_pred γ kA m2 : iProp :=
-  ∃ nA nB kB,
-    ⌜m2 = Spec.of_list [nA; nB; TKey Enc kB]⌝ ∧
-    (pterm nB ↔ ▷ corruption kA kB) ∧
-    session term_meta N γ Resp nA nB (kA, kB).
+Definition nsl_resp : expr :=
+  pk_auth_resp N nsl_gen_keys nsl_mk_sess_key.
 
-Definition msg3_pred γ kB nB : iProp :=
-  ∀ nA kA,
-    session term_meta N γ Resp nA nB (kA, kB) -∗
-    session term_meta N γ Init nA nB (kA, kB) ∧
-    (pterm nA ↔ ▷ corruption kA kB).
+Class NSL := {
+  session : role → term → term → term → iProp;
+}.
 
-Definition nsl_ctx γ : iProp :=
-  session_ctx term_meta N nsl_sess_inv γ ∧
-  enc_pred (N.@"m1") msg1_pred ∧
-  enc_pred (N.@"m2") (msg2_pred γ) ∧
-  enc_pred (N.@"m3") (msg3_pred γ).
+Context `{!NSL}.
 
-Lemma nsl_alloc E E' :
-  ↑N ⊆ E →
-  enc_pred_token E ={E'}=∗ ∃ γ, nsl_ctx γ.
-Proof.
-iIntros (sub) "token".
-iMod (session_alloc term_meta N nsl_sess_inv) as (γ) "#ctx".
-rewrite (enc_pred_token_difference (↑N.@"m1") E); last solve_ndisj.
-iDestruct "token" as "[t1 token]".
-iMod (enc_pred_set (N.@"m1") msg1_pred with "t1") as "#H1" => //.
-rewrite (enc_pred_token_difference (↑N.@"m2")); last solve_ndisj.
-iDestruct "token" as "[t2 token]".
-iMod (enc_pred_set (N.@"m2") (msg2_pred γ) with "t2") as "#H2" => //.
-rewrite (enc_pred_token_difference (↑N.@"m3")); last solve_ndisj.
-iDestruct "token" as "[t3 token]".
-iMod (enc_pred_set (N.@"m3") (msg3_pred γ) with "t3") as "#H3" => //.
-by iModIntro; iExists γ; do !iSplit => //.
+Definition nsl_ctx : iProp :=
+  session.session_ctx (@nonce_meta _ _) N
+    (λ rl nI nR '(kI, kR), session rl kI kR nI).
+
+Definition nsl_resp_accepted kI kR sI sR : iProp :=
+  session.session (@nonce_meta _ heap) N Resp sI sR (kI, kR).
+
+Definition nsl_init_finished sR : iProp := □ ∀ kI kR sI,
+  session.session (@nonce_meta _ _) N Resp sI sR (kI, kR) →
+  session.session (@nonce_meta _ _) N Init sI sR (kI, kR).
+
+Program Instance PK_NSL : PK N := {
+  inv := nsl_ctx;
+
+  init_waiting kI kR nI sI := (
+    ⌜sI = nI⌝ ∧ nonce_meta_token nI (↑N)
+  )%I;
+
+  resp_accepted := nsl_resp_accepted;
+
+  resp_waiting kI kR sI nR sR := (
+    ⌜sR = nR⌝ ∧ nonce_meta_token nR (↑N)
+  )%I;
+
+  init_finished := nsl_init_finished;
+
+  session rl kI kR kS := session rl kI kR kS;
+
+  init_gen_keys := nsl_gen_keys;
+  init_mk_sess_key := nsl_mk_sess_key;
+  resp_gen_keys := nsl_gen_keys;
+  resp_mk_sess_key := nsl_mk_sess_key;
+  
+}.
+
+Next Obligation.
+iIntros "%E %kI %kR % #? !> %Ψ _ post". rewrite /nsl_gen_keys.
+wp_pures. wp_bind (mknonce _).
+iApply (wp_mknonce _ (λ _, corruption kI kR) (λ _, True)%I).
+iIntros "%nI #s_nI #p_nI _ token".
+rewrite (term_meta_token_difference _ (↑N)) //.
+iDestruct "token" as "[token _]".
+wp_pures. iModIntro. iApply "post". do !iSplit; eauto.
+by rewrite /secret_of bi.intuitionistic_intuitionistically.
 Qed.
 
-Global Instance persistent_nsl_ctx γ : Persistent (nsl_ctx γ).
-Proof. apply _. Qed.
+Next Obligation.
+iIntros "%E %kI %kR %nI %sI %sR % #? #accepted %Ψ !> [-> token] post".
 
-Lemma nsl_ctx_session_ctx γ :
-  nsl_ctx γ -∗
-  session_ctx term_meta N nsl_sess_inv γ.
-Proof. by iIntros "( ? & ? )". Qed.
 
-Ltac protocol_failure :=
-  by intros; wp_pures; iApply ("Hpost" $! None).
-
-Definition nsl_init : val := λ: "c" "skA" "pkA" "pkB" "nA",
-  let: "m1"   := tenc (N.@"m1") "pkB" (term_of_list ["nA"; "pkA"]) in
-  send "c" "m1";;
-  bind: "m2"   := tdec (N.@"m2") "skA" (recv "c") in
-  bind: "m2"   := list_of_term "m2" in
-  list_match: ["nA'"; "nB"; "pkB'"] := "m2" in
-  assert: eq_term "nA'" "nA" && eq_term "pkB'" "pkB" in
-  let: "m3" := tenc (N.@"m3") "pkB" "nB" in
-  send "c" "m3";;
-  SOME "nB".
-
-Definition nsl_resp : val := λ: "c" "skB" "pkB" "nB",
-  bind: "m1" := tdec (N.@"m1") "skB" (recv "c") in
-  bind: "m1" := list_of_term "m1" in
-  list_match: ["nA"; "pkA"] := "m1" in
-  bind: "kt" := is_key "pkA" in
-  assert: "kt" = repr Enc in
-  let: "m2" := tenc (N.@"m2") "pkA" (term_of_list ["nA"; "nB"; "pkB"]) in
-  send "c" "m2";;
-  bind: "m3" := tdec (N.@"m3") "skB" (recv "c") in
-  assert: eq_term "m3" "nB" in SOME ("pkA", "nA").
-
-Implicit Types Ψ : val → iProp.
-
-Variable γ : gname.
-
-Lemma pterm_msg1I kA kB (nA : term) :
-  nsl_ctx γ -∗
-  pterm (TKey Enc kA) -∗
-  sterm nA -∗
-  □ (pterm nA ↔ ▷ corruption kA kB) -∗
-  pterm (TKey Enc kB) -∗
-  ▷ pterm (TEnc kB (Spec.tag (N.@"m1") (Spec.of_list [nA; TKey Enc kA]))).
-Proof.
-iIntros "(_ & #Hm1 & _ & _) #HkA #HnA #HnA_hi #HkB".
-iModIntro.
-iApply pterm_TEncIS; eauto.
-- by iApply pterm_sterm.
-- iModIntro.
-  iExists _, _; iSplit; eauto.
-  rewrite sterm_of_list /=; do !iSplit => //.
-  by iApply pterm_sterm.
-- iIntros "!> HkB_dec".
-  rewrite pterm_of_list /=; do !iSplit => //.
-  by iApply "HnA_hi"; rewrite /corruption; eauto.
-Qed.
-
-Lemma pterm_msg2I kA kB nA nB :
-  nsl_ctx γ -∗
-  ▷ pterm (TKey Enc kA) -∗
-  pterm (TKey Enc kB) -∗
-  sterm nA -∗
-  □ (pterm (TKey Dec kA) → pterm nA) -∗
-  sterm nB -∗
-  □ (pterm nB ↔ ▷ corruption kA kB) -∗
-  session term_meta N γ Resp nA nB (kA, kB) -∗
-  ▷ pterm (TEnc kA (Spec.tag (N.@"m2") (Spec.of_list [nA; nB; TKey Enc kB]))).
-Proof.
-iIntros "# (_ & _ & Hm2 & _) #HAenc #HBenc #HnAhi #HnAlo #HnBhi #HnBlo #sess !>".
-iApply pterm_TEncIS; eauto.
-- by iApply pterm_sterm.
-- iModIntro; iExists _, _, _; do ![iSplit => //].
-  rewrite sterm_of_list /=; do !iSplit => //.
-  by iApply pterm_sterm.
-iIntros "!> #pub".
-iSpecialize ("HnAlo" with "pub").
-rewrite pterm_of_list /=; do !iSplit => //.
-by iApply "HnBlo"; rewrite /corruption; eauto.
-Qed.
-
-Lemma pterm_msg1E kA kB nA :
-  nsl_ctx γ -∗
-  pterm (TEnc kB (Spec.tag (N.@"m1") (Spec.of_list [nA; TKey Enc kA]))) -∗
-  ▷ (pterm (TKey Enc kA) ∧ sterm nA ∧
-     (pterm nA ∨ (pterm nA ↔ ▷ corruption kA kB))).
-Proof.
-iIntros "# (_ & m1P & _ & _) #Hts".
-iDestruct (pterm_TEncE with "Hts [//]") as "{Hts} [[HkB Hts]|Hts]".
-  rewrite pterm_of_list /=.
-  iDestruct "Hts" as "(HnA & HkA & _)".
-  iAssert (sterm nA) as "#?". by iApply pterm_sterm.
-  by eauto.
-iDestruct "Hts" as "(#inv & Hts & _)"; iModIntro.
-iDestruct "inv" as (nA' kA') "(%e & HnA & #HkA)".
-move/Spec.of_list_inj: e => [] <- <-.
-rewrite sterm_of_list /=; iDestruct "Hts" as "(? & ? & ?)".
-by eauto.
-Qed.
-
-Lemma pterm_msg2E kA kB nA nB :
-  nsl_ctx γ -∗
-  □ (pterm nA ↔ ▷ corruption kA kB) -∗
-  pterm (TEnc kA (Spec.tag (N.@"m2") (Spec.of_list [nA; nB; TKey Enc kB]))) -∗
-  ▷ (sterm nB ∧
-     (pterm nB ↔ ▷ corruption kA kB) ∧
-     ▷ (corruption kA kB ∨
-        session term_meta N γ Resp nA nB (kA, kB))).
-Proof.
-iIntros "# (_ & _ & ? & _) #p_nA #Hts".
-iDestruct (pterm_TEncE with "Hts [//]") as "{Hts} [[? Hts] | Hts]".
-  rewrite pterm_of_list /=.
-  iDestruct "Hts" as "(p_nA' & ? & ? & ?)".
-  iAssert (sterm nB) as "#?". by iApply pterm_sterm.
-  iPoseProof ("p_nA" with "p_nA'") as "?".
-  by do 3![iSplit; eauto].
-iDestruct "Hts" as "(#inv & Hts & _)"; iModIntro.
-iDestruct "inv" as (nA' nB' kB') "(%e_m & #nBP & frag)".
-case/Spec.of_list_inj: e_m => <- <- <-; rewrite sterm_of_list /=.
-iDestruct "Hts" as "(?&?&?)"; by eauto.
-Qed.
-
-Lemma pterm_msg3I kA kB nA nB :
-  nsl_ctx γ -∗
-  pterm (TKey Enc kA) -∗
-  pterm (TKey Enc kB) -∗
-  □ (pterm nA ↔ ▷ corruption kA kB) -∗
-  sterm nB -∗
-  □ (pterm nB ↔ ▷ corruption kA kB) -∗
-  session term_meta N γ Resp nA nB (kA, kB) -∗
-  session term_meta N γ Init nA nB (kA, kB) -∗
-  pterm (TEnc kB (Spec.tag (N.@"m3") nB)).
-Proof.
-iIntros "(_ & _ & _ & #Hm3) #p_kA #p_kB #p_nA #s_nB #p_nB #sessA #sessB".
-iApply pterm_TEncIS => //.
-- by iApply pterm_sterm.
-- iModIntro. iIntros (nA' kA') "#sessA'".
-  iDestruct (session_agree with "sessA sessA'") as "(<- & %e)" => //.
-  case: e => <-.
-  by iSplit.
-by iIntros "!> ?"; iApply "p_nB"; rewrite /corruption; eauto.
-Qed.
-
-Lemma pterm_msg3E kA kB nA nB :
-  nsl_ctx γ -∗
-  session term_meta N γ Resp nA nB (kA, kB) -∗
-  □ (pterm nB ↔ ▷ corruption kA kB) -∗
-  pterm (TEnc kB (Spec.tag (N.@"m3") nB)) -∗
-  ▷ (corruption kA kB ∨
-     session term_meta N γ Init nA nB (kA, kB) ∧
-     (pterm nA ↔ ▷ corruption kA kB)).
-Proof.
-iIntros "(_ & _ & _ & #Hm3) #sessB #p_nB #p_m3".
-iDestruct (pterm_TEncE with "p_m3 [//]") as "[[_ fail]|inv]".
-  by iLeft; iApply "p_nB".
-iDestruct "inv" as "(#inv & _ & _)".
-iModIntro; iRight.
-by iApply "inv".
-Qed.
-
-Lemma wp_nsl_init c kA kB (nA : term) E Ψ :
-  ↑cryptisN ⊆ E →
-  ↑N ⊆ E →
-  channel c -∗
-  nsl_ctx γ -∗
-  pterm (TKey Enc kA) -∗
-  pterm (TKey Enc kB) -∗
-  sterm nA -∗
-  □ (pterm nA ↔ ▷ corruption kA kB) -∗
-  (∀ nB, |==> P Init nA nB kA kB ∗ Q Init nA nB kA kB) -∗
-  term_meta_token nA (↑N) -∗
-  (∀ onB : option term,
-      (if onB is Some nB then
-         sterm nB ∧
-         Q Init nA nB kA kB ∗
-         (corruption kA kB ∨ P Resp nA nB kA kB)
-       else True) -∗
-      Ψ (repr onB)) -∗
-  WP nsl_init c (TKey Dec kA) (TKey Enc kA) (TKey Enc kB) nA @ E
-     {{ Ψ }}.
-Proof.
-rewrite /nsl_init.
-iIntros (??) "#c #ctx #enc_kA #enc_kB #s_nA #p_nA inv unreg Hpost".
-wp_list; wp_term_of_list.
-wp_tenc => /=.
-iPoseProof (pterm_msg1I with "[//] enc_kA s_nA p_nA enc_kB") as "#Hm1".
-wp_pures; wp_bind (send _ _); iApply wp_send; eauto.
-iClear "Hm1"; wp_pures; wp_bind (recv _); iApply wp_recv => //.
-iIntros (m2) "#Hm2"; wp_tdec m2; last protocol_failure.
-wp_list_of_term m2; last protocol_failure.
-wp_list_match => [nA' nB pkB' {m2} ->|_]; last protocol_failure.
-wp_eq_term e; last protocol_failure; subst nA'.
-wp_eq_term e; last protocol_failure; subst pkB'.
-wp_tenc.
-iPoseProof (pterm_msg2E with "[//] [//] Hm2")
-  as "{Hm2} (s_nB & p_nB & Hm2)"; eauto.
-iMod ("inv" $! nB) as "[HP HQ]".
-wp_pures; iDestruct "Hm2" as "[fail|sessB]".
-  wp_bind (send _ _); iApply wp_send => //.
-    iApply pterm_TEncIP => //.
-    by rewrite pterm_tag; iApply "p_nB".
-  wp_pures; iApply ("Hpost" $! (Some nB)); eauto.
-  iModIntro; by iSplit => //; iFrame; eauto.
-iMod (session_begin _ γ Init _ _ (kA, kB)
-        with "[] [HP] [unreg]") as "[#sessA close]" => //.
-- by iApply nsl_ctx_session_ctx.
-- by eauto.
-iMod ("close" with "sessB") as "inv_resp" => //=.
-wp_bind (send _ _); iApply wp_send => //.
-  by iApply (pterm_msg3I with "[] [] [] [] [] [] sessB sessA"); eauto.
-wp_pures; iApply ("Hpost" $! (Some nB)); eauto.
-iModIntro; by iSplit => //; iFrame; eauto.
-Qed.
-
-Lemma wp_nsl_resp c kB E Ψ nB :
-  ↑cryptisN ⊆ E →
-  ↑N ⊆ E →
-  channel c -∗
-  nsl_ctx γ -∗
-  pterm (TKey Enc kB) -∗
-  term_meta_token nB (↑N) -∗
-  sterm nB -∗
-  (∀ kA nA, |==> □ (pterm nB ↔ ▷ corruption kA kB) ∗
-                 P Resp nA nB kA kB ∗ Q Resp nA nB kA kB
-  ) -∗
-  (∀ ot : option (term * term),
-      (if ot is Some (pkA, nA) then
-         ∃ kA,
-           ⌜pkA = TKey Enc kA⌝ ∧
-           pterm pkA ∧
-           sterm nA ∧
-           □ (pterm nA ↔ ▷ corruption kA kB) ∧
-           Q Resp nA nB kA kB ∗
-           (corruption kA kB ∨ P Init nA nB kA kB)
-       else True) -∗
-       Ψ (repr ot)) -∗
-  WP nsl_resp c (TKey Dec kB) (TKey Enc kB) nB @ E {{ Ψ }}.
-Proof.
-iIntros (??) "#? #ctx #e_kB unreg #s_nB set_nB Hpost".
-rewrite /nsl_resp; wp_pures.
-wp_bind (recv _); iApply wp_recv => //; iIntros (m1) "#Hm1".
-wp_tdec m1; last protocol_failure.
-wp_list_of_term m1; last protocol_failure.
-wp_list_match => [nA pkA {m1} ->|_]; last protocol_failure.
-wp_is_key_eq kt kA et; last protocol_failure; subst pkA.
-wp_pures.
-case: (bool_decide_reflect (_ = repr_key_type Enc)); last protocol_failure.
-case: kt => // _.
-wp_pures.
-iDestruct (pterm_msg1E with "[] Hm1") as "{Hm1} Hm1"; eauto.
-wp_list; wp_term_of_list.
-iMod ("set_nB" $! kA nA) as "[#p_nB [HP HQ]]".
-wp_tenc; wp_pures.
-iDestruct "Hm1" as "(e_kA & s_nA & Hm1)".
-iAssert (□ (▷ corruption kA kB → pterm nA))%I as "#p_nA".
-  iDestruct "Hm1" as "[?|#e]"; eauto.
-  by iIntros "!> ?"; iApply "e"; eauto.
-iMod (session_begin _ γ Resp _ _ (kA, kB)
-       with "[] [HP] [unreg]") as "[#sessB close]" => //.
-- by iApply nsl_ctx_session_ctx.
-- by [].
-iPoseProof (pterm_msg2I with "[//] [//] e_kB s_nA [] s_nB [] sessB") as "Hm2".
-- by iIntros "!> ?"; iApply "p_nA"; rewrite /corruption; eauto.
-- by eauto.
-wp_bind (send _ _); iApply wp_send => //.
-wp_pures; wp_bind (recv _); iApply wp_recv => //; iIntros (m3) "#Hm3".
-wp_tdec m3; last protocol_failure.
-wp_eq_term e; last protocol_failure; subst m3.
-iPoseProof (pterm_msg3E with "[] sessB p_nB []") as "[pub|sec]" => //.
-  iSpecialize ("p_nB" with "pub").
-  wp_pures. iApply ("Hpost" $! (Some (TKey Enc kA, nA))).
-  iModIntro; iExists kA; do 4!iSplit => //.
-    iModIntro; iSplit; iIntros "#?" => //.
-    iDestruct "Hm1" as "[?|#Hm1]"; eauto.
-    by iApply "Hm1".
-  iFrame; by iLeft.
-iDestruct "sec" as "{p_nA} (sessA & p_nA)".
-wp_if.
-iMod ("close" with "sessA") as "inv".
-wp_pures.
-iApply ("Hpost" $! (Some (TKey Enc kA, nA))).
-iExists kA; iModIntro; do 4!iSplit => //; eauto.
-by iFrame; eauto.
-Qed.
 
 End NSL.
 
