cryptis.v
@@ -3,7 +3,7 @@ From stdpp Require Import gmap.
 From iris.algebra Require Import agree auth gset gmap list reservation_map.
 From iris.base_logic.lib Require Import saved_prop.
 From iris.heap_lang Require Import notation proofmode.
-From cryptis Require Import lib term.
+From cryptis Require Import lib term nown.
 
 Set Implicit Arguments.
 Unset Strict Implicit.
@@ -17,9 +17,10 @@ Class cryptisG Σ := CryptisG {
   cryptis_inG       :> savedPredG Σ term;
   cryptis_key_inG   :> savedPredG Σ (key_type * term);
   cryptis_enc_inG   :> savedPredG Σ (term * term);
-  cryptis_key_name : gname;
+  cryptis_nown      :> nownGS;
+  cryptis_key_name  : gname;
   cryptis_hash_name : gname;
-  cryptis_enc_name : gname;
+  cryptis_enc_name  : gname;
 }.
 
 Definition cryptisΣ : gFunctors :=
@@ -845,7 +846,7 @@ End Cryptis.
 Lemma cryptisG_alloc `{!heapGS Σ} :
   cryptisPreG Σ →
   ⊢ |==> ∃ (H : cryptisG Σ),
-           enc_pred_token ⊤ ∗ key_pred_token ⊤ ∗ hash_pred_token ⊤.
+           enc_pred_token ⊤ ∗ key_pred_token ⊤ ∗ hash_pred_token ⊤ ∗ nown_token ⊤.
 Proof.
 move=> ?; iStartProof.
 iMod (own_alloc (reservation_map_token ⊤)) as (γ_enc) "own_enc".
@@ -854,8 +855,9 @@ iMod (own_alloc (reservation_map_token ⊤)) as (γ_key) "own_key".
   apply reservation_map_token_valid.
 iMod (own_alloc (reservation_map_token ⊤)) as (γ_hash) "own_hash".
   apply reservation_map_token_valid.
+iMod (nownGS_alloc) as "(% & own_nown)".
 iModIntro.
-by iExists (CryptisG _ _ _ γ_enc γ_key γ_hash); iFrame.
+by iExists (CryptisG _ _ _ _ γ_enc γ_key γ_hash); iFrame.
 Qed.
 
 Arguments cryptis_enc_name {Σ _}.
