nown.v
@@ -1,0 +1,130 @@
+(* A global map from namespaces to ghost names. *)
+
+From stdpp Require Import base gmap.
+From mathcomp Require Import ssreflect.
+From iris.algebra Require Import agree auth csum gset gmap reservation_map.
+From iris.heap_lang Require Import notation proofmode.
+From cryptis Require Import lib.
+
+Set Implicit Arguments.
+Unset Strict Implicit.
+Unset Printing Implicit Defensive.
+
+Section NOwn.
+
+Context `{!heapGS Σ}.
+Notation iProp := (iProp Σ).
+
+Class nownGS := {
+  nownGS_name : gname;
+}.
+
+Context `{!nownGS}.
+
+Definition nown_token E : iProp :=
+  own nownGS_name (reservation_map_token E).
+
+Definition nown_name N (γ : gname) : iProp :=
+  own nownGS_name (namespace_map_data N (to_agree γ)).
+
+#[global]
+Instance nown_name_timeless N γ : Timeless (nown_name N γ).
+Proof. apply _. Qed.
+
+#[global]
+Instance nown_name_persistent N γ : Persistent (nown_name N γ).
+Proof. apply _. Qed.
+
+Lemma nown_name_set E N γ :
+  ↑N ⊆ E →
+  nown_token E ==∗ nown_name N γ.
+Proof.
+iIntros (?) "token".
+iMod (own_update with "token") as "data".
+  by apply (namespace_map_alloc_update _ N (to_agree γ)).
+by eauto.
+Qed.
+
+Lemma nown_name_agree N γ1 γ2 :
+  nown_name N γ1 -∗
+  nown_name N γ2 -∗
+  ⌜γ1 = γ2⌝.
+Proof.
+iIntros "own1 own2".
+iPoseProof (own_valid_2 with "own1 own2") as "%valid".
+move: valid; rewrite -reservation_map_data_op reservation_map_data_valid.
+by move=> /to_agree_op_inv_L ->.
+Qed.
+
+Lemma nown_token_difference E1 E2 :
+  E1 ⊆ E2 →
+  nown_token E2 ⊣⊢ nown_token E1 ∗ nown_token (E2 ∖ E1).
+Proof.
+move=> ?.
+by rewrite /nown_token -own_op -reservation_map_token_difference.
+Qed.
+
+Definition nown `{!inG Σ A} N (a : A) : iProp :=
+  ∃ γ, nown_name N γ ∧ own γ a.
+
+Lemma nown_alloc `{!inG Σ A} N E (a : A) :
+  ↑N ⊆ E → ✓ a → nown_token E ==∗ nown N a.
+Proof.
+intros sub valid_a. iIntros "token".
+iMod (own_alloc a) as "(%γ & own)"; auto.
+iMod (nown_name_set γ with "token") as "name"; eauto.
+iModIntro. iExists γ. eauto.
+Qed.
+
+Lemma nown_valid `{!inG Σ A} N (a : A) : nown N a -∗ ✓ a.
+Proof.
+iIntros "(%γ & #own_γ & own)". iApply (own_valid with "own").
+Qed.
+
+Lemma nown_valid_2 `{!inG Σ A} N (a1 a2 : A) :
+  nown N a1 -∗ nown N a2 -∗ ✓ (a1 ⋅ a2).
+Proof.
+iIntros "(%γ & #own_γ & own1) (%γ' & own_γ' & own2)".
+iPoseProof (nown_name_agree with "own_γ own_γ'") as "<-".
+by iApply (own_valid_2 with "own1 own2").
+Qed.
+
+Lemma nown_update `{!inG Σ A} N (a a' : A) : a ~~> a' → nown N a ==∗ nown N a'.
+Proof.
+iIntros (?) "(%γ & #? & own)".
+iMod (own_update with "own") as "own"; eauto.
+iModIntro. iExists γ. eauto.
+Qed.
+
+#[global]
+Instance nown_core_persistent `{!inG Σ A} N (a : A) :
+  CoreId a → Persistent (nown N a).
+Proof. apply _. Qed.
+
+#[global]
+Instance nown_timeless `{!inG Σ A} N (a : A) :
+  Discrete a → Timeless (nown N a).
+Proof. apply _. Qed.
+
+Lemma nown_op `{!inG Σ A} N (a1 a2 : A) :
+  nown N (a1 ⋅ a2) ⊣⊢ nown N a1 ∗ nown N a2.
+Proof.
+iSplit.
+- iIntros "(%γ & #? & [own1 own2])".
+  by iSplitL "own1"; iExists γ; iSplit.
+- iIntros "[(%γ & #own_γ & own1) (%γ' & #own_γ' & own2)]".
+  iPoseProof (nown_name_agree with "own_γ own_γ'") as "<-".
+  iExists γ. iSplit => //. by iSplitL "own1".
+Qed.
+
+End NOwn.
+
+Lemma nownGS_alloc `{!heapGS Σ} : ⊢ |==> ∃ (H : nownGS), nown_token ⊤.
+Proof.
+iMod (own_alloc (reservation_map_token ⊤)) as "(%γ & own)".
+  apply reservation_map_token_valid.
+iModIntro.
+by iExists (Build_nownGS γ).
+Qed.
+
+Arguments nown_alloc {Σ _ _ A _} N {_} a.
